compiler/backend/stackLangScript.sml
@@ -52,6 +52,7 @@ val _ = map overload_on
    ("sub_1_inst",``\r1. Inst (Arith (Binop Sub r1 r1 (Imm 1w)))``),
    ("sub_inst",``\r1 r2. Inst (Arith (Binop Sub r1 r1 (Reg r2)))``),
    ("add_inst",``\r1 r2. Inst (Arith (Binop Add r1 r1 (Reg r2)))``),
+   ("and_inst",``\r1 r2. Inst (Arith (Binop And r1 r1 (Reg r2)))``),
    ("add_1_inst",``\r1. Inst (Arith (Binop Add r1 r1 (Imm 1w)))``),
    ("or_inst",``\r1 r2. Inst (Arith (Binop Or r1 r1 (Reg r2)))``),
    ("add_bytes_in_word_inst",``\r1. Inst (Arith (Binop Add r1 r1 (Imm (bytes_in_word))))``),
